Cleaned-up names and Organization

Examples/GodelT_norm/GodelT_norm.lean
@@ -3,7 +3,7 @@ import Mathlib.Tactic
 -- From: https://cs.ioc.ee/ewscs/2009/dybjer/mainPalmse-revised.pdf
 
 inductive Ty : Type
-| Nat : Ty
+| nat : Ty
 | arrow : Ty → Ty → Ty
 open Ty
 infixr : 100 " ⇒' " => arrow
@@ -11,40 +11,40 @@ infixr : 100 " ⇒' " => arrow
 inductive Exp : Ty → Type
 | K {a b : Ty}     :  Exp (a ⇒' b ⇒' a)
 | S {a b c : Ty}   :  Exp ((a ⇒' b ⇒' c) ⇒' (a ⇒' b) ⇒' (a ⇒' c))
-| App {a b : Ty}   :  Exp (a ⇒' b) → Exp a → Exp b
-| zero             :  Exp Nat
-| succ             :  Exp (Nat ⇒' Nat)
-| recN {a : Ty}    :  Exp (a ⇒' (Nat ⇒' a ⇒' a) ⇒' Nat ⇒' a)
+| app {a b : Ty}   :  Exp (a ⇒' b) → Exp a → Exp b
+| zero             :  Exp nat
+| succ             :  Exp (nat ⇒' nat)
+| recN {a : Ty}    :  Exp (a ⇒' (nat ⇒' a ⇒' a) ⇒' nat ⇒' a)
 open Exp
-infixl : 100 " ⬝ " => App
+infixl : 100 " ⬝ " => app
 
 -- Didn't declare Setoid instance yet
-inductive convr : Π {α : Ty}, (Exp α) → (Exp α) → Prop
+inductive R : Π {α : Ty}, (Exp α) → (Exp α) → Prop
 | refl {α : Ty}{e : Exp α}
-        : convr (e) (e)
-| sym   {α : Ty}{e e' : Exp α}
-        : convr (e) (e') → convr (e') (e)
+        : R (e) (e)
+| symm   {α : Ty}{e e' : Exp α}
+        : R (e) (e') → R (e') (e)
 | trans {α : Ty}{e e' e'' : Exp α}
-        : convr (e) (e') → convr (e') (e'') → convr (e) (e'')
+        : R (e) (e') → R (e') (e'') → R (e) (e'')
 | K     {α β : Ty}{x : Exp α} {y : Exp β}
-        : convr (K ⬝ x ⬝ y) (x)
+        : R (K ⬝ x ⬝ y) (x)
 | S     {α β γ: Ty}{x : Exp (γ ⇒' β ⇒' α)} {y : Exp (γ ⇒' β)} {z : Exp γ}
-        : convr (S ⬝ x ⬝ y ⬝ z) (x ⬝ z ⬝ (y ⬝ z))
+        : R (S ⬝ x ⬝ y ⬝ z) (x ⬝ z ⬝ (y ⬝ z))
 | app   {α β : Ty} {a b : Exp (β ⇒' α)} {c d : Exp β}
-        : convr (a) (b) → convr (c) (d) → convr (a ⬝ c) (b ⬝ d)
-| recN_zero {α : Ty} {e : Exp α} {f : Exp (Nat ⇒' α ⇒' α)}
-        : convr (recN ⬝ e ⬝ f ⬝ zero) (e)
-| recN_succ {α : Ty} {n : Exp Nat} {e : Exp α} {f : Exp (Nat ⇒' α ⇒' α)}
-        : convr (recN ⬝ e ⬝ f ⬝ (succ ⬝ n)) (f ⬝ n ⬝ (recN ⬝ e ⬝ f ⬝ n))
+        : R (a) (b) → R (c) (d) → R (a ⬝ c) (b ⬝ d)
+| recN_zero {α : Ty} {e : Exp α} {f : Exp (nat ⇒' α ⇒' α)}
+        : R (recN ⬝ e ⬝ f ⬝ zero) (e)
+| recN_succ {α : Ty} {n : Exp nat} {e : Exp α} {f : Exp (nat ⇒' α ⇒' α)}
+        : R (recN ⬝ e ⬝ f ⬝ (succ ⬝ n)) (f ⬝ n ⬝ (recN ⬝ e ⬝ f ⬝ n))
 
 
 def Ty_inter : Ty → Type
-| Ty.Nat => ℕ
+| nat => ℕ
 
 | arrow a b => Exp (a ⇒' b) × (Ty_inter a → Ty_inter b)
 
 
-def numeral : ℕ → Exp Ty.Nat
+def numeral : ℕ → Exp nat
 | 0 => zero
 
 | n+1 => succ ⬝ (numeral n)
@@ -52,7 +52,7 @@ def numeral : ℕ → Exp Ty.Nat
 
 def reify (α : Ty) (e : Ty_inter α) : Exp α :=
   match α,e with
-  | Ty.Nat, e            => numeral e
+  | nat, e            => numeral e
 
   | Ty.arrow α β, (c, f) => c
 
@@ -68,13 +68,13 @@ def Exp_inter (a : Ty) : (e : Exp a) → Ty_inter a
               (λ x ↦ (S ⬝ (reify (a⇒'b⇒'c) x),
               (λ y ↦ (S ⬝ (reify (a⇒'b⇒'c) x) ⬝ (reify (a⇒'b) y),
               (λ z ↦ appsem (appsem x z) (appsem y z)))))))
-| @App a b f e  => appsem (Exp_inter (a ⇒' b) f) (Exp_inter a e)
+| @app a b f e  => appsem (Exp_inter (a ⇒' b) f) (Exp_inter a e)
 | zero          => (0 : ℕ)
 | succ          => (succ,
                    (λ n : ℕ ↦ n+1) )
 | @recN a       => (recN,
                    (λ p ↦ (recN ⬝ (reify a p),
-                   (λ q ↦ (recN ⬝ (reify a p) ⬝ (reify (Nat⇒'a⇒'a) q),
+                   (λ q ↦ (recN ⬝ (reify a p) ⬝ (reify (nat⇒'a⇒'a) q),
                    (λ n0 ↦ Nat.rec p (λ n r ↦ appsem (appsem q n) r) n0))))))
 
 
@@ -82,7 +82,7 @@ def nbe (a : Ty) (e : Exp a) : (Exp a) := reify a (Exp_inter a e)
 
 
 -- e ~ e'  implies [[e]]a = [[e']]a
-lemma convr_lemma1 {a : Ty} {e e' : Exp a} : convr e e' → ((Exp_inter a e) = (Exp_inter a e')) :=
+lemma R_lemma1 {a : Ty} {e e' : Exp a} : R e e' → ((Exp_inter a e) = (Exp_inter a e')) :=
 by
   intro h
   induction h
@@ -92,188 +92,189 @@ by
     rw [ab_ih, cd_ih]
 
 -- e ~ e'  implies nbe a e = nbe a e'
-lemma soundness {a : Ty} {e e' : Exp a} : convr e e' → nbe a e = nbe a e' :=
+lemma soundness {a : Ty} {e e' : Exp a} : R e e' → nbe a e = nbe a e' :=
 by
   unfold nbe
   intro h1
-  have h2 : Exp_inter a e = Exp_inter a e' := convr_lemma1 h1
+  have h2 : Exp_inter a e = Exp_inter a e' := R_lemma1 h1
   rw [h2]
 
 
 -- Tait-reducibility relation
-def R : (a : Ty) → (e : Exp a) → Prop
-| Ty.Nat, e       => convr e (nbe Ty.Nat e)
+def Red : (a : Ty) → (e : Exp a) → Prop
+| nat, e       => R e (nbe nat e)
 
-| Ty.arrow α β, e => convr e (nbe (α ⇒' β) e)  ∧  ∀ e', R α e' → R β (App e e')
+| arrow α β, e => R e (nbe (α ⇒' β) e)  ∧  ∀ e', Red α e' → Red β (app e e')
 
 -- R a e  implies  e ~ nbe a e
-lemma R_convr_nbe (h : R a e)  : convr e (nbe a e) :=
+lemma Red_R_nbe (h : Red a e)  : R e (nbe a e) :=
   by
   cases a
-  all_goals (unfold R at h); aesop
+  all_goals (unfold Red at h); aesop
 
 -- e ~ e' implies  R α e ↔ R α e'
-lemma convr_R_iff : ∀ e e', convr e e' → (R α e ↔ R α e') :=
+lemma Red_resp : ∀ e e', R e e' → (Red α e = Red α e') :=
   by
+  refine fun e e' a ↦ ?_ ; apply propext ; revert a e' e
   induction α
-  · unfold R
+  · unfold Red
     intro a b a_r_b
     apply Iff.intro
     · intro a_r_nbe
-      --convr-rewriting here:
+      --R-rewriting here:
       -- b ~ a ~ nbe a = nbe b
       -- "rewrite [← a_r_b, a_r_nbe, soundness a_r_b]"
-      have eq : nbe Ty.Nat a = nbe Ty.Nat b := soundness a_r_b
+      have eq : nbe nat a = nbe nat b := soundness a_r_b
       (rewrite [← eq]); clear eq
-      apply convr.trans (a_r_b).sym
+      apply R.trans (a_r_b).symm
       exact a_r_nbe
     · intro b_r_nbe
-      --convr-rewriting here:
+      --R-rewriting here:
       -- a ~ b ~ nbe b = nbe a
       -- "rewrite [a_r_b, b_r_nbe, ← soundness a_r_b]"
-      have eq : nbe Ty.Nat a = nbe Ty.Nat b := soundness a_r_b
+      have eq : nbe nat a = nbe nat b := soundness a_r_b
       (rewrite [eq]); clear eq
-      exact convr.trans a_r_b b_r_nbe
+      exact R.trans a_r_b b_r_nbe
 
   · rename_i α β _ βIH
     intros f1 f2 f1_r_f2
     apply Iff.intro
     · intro R_f1
       apply And.intro
-      · have f1_r_nbe := R_convr_nbe R_f1; clear R_f1
-        -- convr-rewriting here:
+      · have f1_r_nbe := Red_R_nbe R_f1; clear R_f1
+        -- R-rewriting here:
         -- f2 ~ f1 ~ nbe f1 = nbe f2
         -- "rewrite [← f1_r_f2, f1_r_nbe, soundness f1_r_f2]"
         have eq : nbe (α ⇒' β) f1 = nbe (α ⇒' β) f2 := soundness f1_r_f2
         rewrite [← eq]; clear eq
-        refine convr.trans ?_ f1_r_nbe
-        exact f1_r_f2.sym
+        refine R.trans ?_ f1_r_nbe
+        exact f1_r_f2.symm
       · intro e' Re'
-        rewrite [← βIH (f1 ⬝ e') (f2 ⬝ e') (f1_r_f2.app convr.refl)]
+        rewrite [← βIH (f1 ⬝ e') (f2 ⬝ e') (f1_r_f2.app R.refl)]
         rcases R_f1 with ⟨_, h0⟩
         exact h0 e' Re'
 
     · intro R_f2
       apply And.intro
-      · have f2_r_nbe := R_convr_nbe R_f2; clear R_f2
-        -- convr-rewriting here:
+      · have f2_r_nbe := Red_R_nbe R_f2; clear R_f2
+        -- R-rewriting here:
         -- f1 ~ f2 ~ nbe f2 = nbe f1
         -- "rewrite [f1_r_f2, f2_r_nbe, ← soundness f1_r_f2]"
         have eq : nbe (α ⇒' β) f1 = nbe (α ⇒' β) f2 := soundness f1_r_f2
         rewrite [eq]; clear eq
         exact f1_r_f2.trans f2_r_nbe
       · intro e' Re'
-        rewrite [βIH (f1 ⬝ e') (f2 ⬝ e') (f1_r_f2.app convr.refl)]
+        rewrite [βIH (f1 ⬝ e') (f2 ⬝ e') (f1_r_f2.app R.refl)]
         rcases R_f2 with ⟨_, h0⟩
         exact h0 e' Re'
 
-lemma R_numeral : R Ty.Nat (numeral n) :=
+lemma Red_numeral : Red nat (numeral n) :=
   by
-  unfold R
+  unfold Red
   induction n
-  case zero => exact convr.refl
+  case zero => exact R.refl
 
   case succ n' IH =>
     unfold numeral
-    -- convr-rewriting here
+    -- R-rewriting here
     -- succ ⬝ numeral n' ~ succ ⬝ nbe (numeral n') = nbe (succ ⬝ numeral n')
     -- "rewrite [IH, nbe]"
-    have eq : nbe Ty.Nat (succ ⬝ numeral n') = succ ⬝ (nbe Ty.Nat $ numeral n') := rfl; rewrite [eq]; clear eq
-    apply (convr.refl).app
+    have eq : nbe nat (succ ⬝ numeral n') = succ ⬝ (nbe nat $ numeral n') := rfl; rewrite [eq]; clear eq
+    apply (R.refl).app
     exact IH
 
--- for all e, R a e
-lemma all_R {e : Exp a} : R a e :=
+-- for all e, Red a e
+lemma all_Red {e : Exp a} : Red a e :=
   by
   induction e
   all_goals clear a
   case K a b =>
     apply And.intro
-    · exact convr.refl
+    · exact R.refl
     · intro e' Re'
       apply And.intro
-      · have e'_r_nbe := R_convr_nbe Re'; clear Re'
-        -- convr-rewriting here
+      · have e'_r_nbe := Red_R_nbe Re'; clear Re'
+        -- R-rewriting here
         -- K ⬝ e' ~ K ⬝ nbe e' = nbe (K ⬝ e')
         -- "rewrite [e'_r_nbe, nbe]"
         have eq : nbe (b ⇒' a) (K ⬝ e') = K ⬝ nbe a e' := rfl; rewrite [eq]; clear eq
-        apply convr.app convr.refl
+        apply R.app R.refl
         exact e'_r_nbe
       · intro e'' _
-        --convr-rewriting here
+        --R-rewriting here
         -- R (K ⬝ e' ⬝ e'') = R e'
-        -- "rewrite [convr.K]"
-        rewrite [convr_R_iff (K ⬝ e' ⬝ e'') e' convr.K]
+        -- "rewrite [R.K]"
+        rewrite [Red_resp (K ⬝ e' ⬝ e'') e' R.K]
         exact Re'
 
   case S a b c =>
     apply And.intro
-    · exact convr.refl
+    · exact R.refl
     · intro x Rx
       apply And.intro
       · have eq : nbe ((a ⇒' b) ⇒' a ⇒' c) (S ⬝ x) = S ⬝ nbe (a ⇒' b ⇒' c)  x := rfl; rewrite [eq]; clear eq
-        -- convr-rewriting here
-        apply convr.app convr.refl
-        exact R_convr_nbe Rx
+        -- R-rewriting here
+        apply R.app R.refl
+        exact Red_R_nbe Rx
       · intro y Ry
         apply And.intro
         · have eq : nbe (a ⇒' c) (S ⬝ x ⬝ y) = S ⬝ nbe (a ⇒' b ⇒' c) x ⬝ nbe (a ⇒' b) y := rfl; rewrite [eq]; clear eq
-          replace Rx := R_convr_nbe Rx; replace Ry := R_convr_nbe Ry
-          -- convr-rewriting here
-          have Sx_r_S_nbex : convr (S ⬝ x) (S ⬝ (nbe (a ⇒' b ⇒' c) x)) := (convr.refl).app Rx
+          replace Rx := Red_R_nbe Rx; replace Ry := Red_R_nbe Ry
+          -- R-rewriting here
+          have Sx_r_S_nbex : R (S ⬝ x) (S ⬝ (nbe (a ⇒' b ⇒' c) x)) := (R.refl).app Rx
           exact Sx_r_S_nbex.app Ry
         · intro z Rz
-          -- convr-rewriting here
-          apply (convr_R_iff (S ⬝ x ⬝ y ⬝ z) _ convr.S).mpr
+          -- R-rewriting here
+          apply (Red_resp (S ⬝ x ⬝ y ⬝ z) _ R.S).mpr
           rcases Rx with ⟨_, Rxz⟩; specialize Rxz z Rz
           rcases Ry with ⟨_, Ryz⟩; specialize Ryz z Rz
           rcases Rxz with ⟨_, Rxzyz⟩; specialize Rxzyz (y ⬝ z) Ryz
           exact Rxzyz
 
-  case App α β f x Rf Rx =>
+  case app α β f x Rf Rx =>
     rcases Rf with ⟨_, h0⟩
     exact h0 x Rx
 
   case zero =>
-    exact convr.refl
+    exact R.refl
 
   case succ =>
     apply And.intro
-    · exact convr.refl
+    · exact R.refl
     · intro x Rx
-      unfold R
-      have eq : nbe Ty.Nat (succ ⬝ x) = succ ⬝ (nbe Ty.Nat x) := rfl; rewrite [eq]; clear eq
-      -- convr-rewriting here
-      exact (convr.refl).app Rx
+      unfold Red
+      have eq : nbe nat (succ ⬝ x) = succ ⬝ (nbe nat x) := rfl; rewrite [eq]; clear eq
+      -- R-rewriting here
+      exact (R.refl).app Rx
 
   case recN α =>
     apply And.intro
-    · exact convr.refl
+    · exact R.refl
     · intro e' Re'
       apply And.intro
-      · have eq : nbe ((Ty.Nat ⇒' α ⇒' α) ⇒' Ty.Nat ⇒' α) (recN ⬝ e') = recN ⬝ nbe α e' := rfl; rewrite [eq]; clear eq
-        -- convr-rewriting here
-        apply convr.app convr.refl
-        exact R_convr_nbe Re'
+      · have eq : nbe ((nat ⇒' α ⇒' α) ⇒' nat ⇒' α) (recN ⬝ e') = recN ⬝ nbe α e' := rfl; rewrite [eq]; clear eq
+        -- R-rewriting here
+        apply R.app R.refl
+        exact Red_R_nbe Re'
       · intro e'' Re''
         apply And.intro
-        · have eq : nbe (Ty.Nat ⇒' α) (recN ⬝ e' ⬝ e'') = recN ⬝ nbe α e' ⬝ nbe (Ty.Nat ⇒' α ⇒' α) e'' := rfl; rewrite [eq]; clear eq
-          replace Re' := R_convr_nbe Re'; replace Re'' := R_convr_nbe Re''
-          -- convr-rewriting here
-          have h0 : convr (recN ⬝ e') (recN ⬝ nbe α e') := (convr.refl).app Re'
+        · have eq : nbe (nat ⇒' α) (recN ⬝ e' ⬝ e'') = recN ⬝ nbe α e' ⬝ nbe (nat ⇒' α ⇒' α) e'' := rfl; rewrite [eq]; clear eq
+          replace Re' := Red_R_nbe Re'; replace Re'' := Red_R_nbe Re''
+          -- R-rewriting here
+          have h0 : R (recN ⬝ e') (recN ⬝ nbe α e') := (R.refl).app Re'
           exact h0.app Re''
         · intro n Rn
           have n_r_nbe := Rn; unfold R at n_r_nbe
           -- "rewrite [n_r_nbe]"
-          rewrite [convr_R_iff (recN ⬝ e' ⬝ e'' ⬝ n) (recN ⬝ e' ⬝ e'' ⬝ (nbe Ty.Nat n)) (convr.refl.app n_r_nbe)]
+          rewrite [Red_resp (recN ⬝ e' ⬝ e'' ⬝ n) (recN ⬝ e' ⬝ e'' ⬝ (nbe nat n)) (R.refl.app n_r_nbe)]
           unfold nbe; simp [reify]
-          induction ((Exp_inter Ty.Nat n))
+          induction ((Exp_inter nat n))
           · unfold numeral
-            -- convr-rewriting here
-            exact (convr_R_iff (recN ⬝ e' ⬝ e'' ⬝ zero) e' convr.recN_zero).mpr Re'
+            -- R-rewriting here
+            exact (Red_resp (recN ⬝ e' ⬝ e'' ⬝ zero) e' R.recN_zero).mpr Re'
           · rename_i n' IH
-            apply (convr_R_iff (.recN ⬝ e' ⬝ e'' ⬝ (.succ ⬝ numeral n')) (e'' ⬝ (numeral n') ⬝ (.recN ⬝ e' ⬝ e'' ⬝ (numeral n'))) convr.recN_succ).mpr
-            have R_numeral_n' : R Ty.Nat (numeral n') := by exact R_numeral
+            apply (Red_resp (.recN ⬝ e' ⬝ e'' ⬝ (.succ ⬝ numeral n')) (e'' ⬝ (numeral n') ⬝ (.recN ⬝ e' ⬝ e'' ⬝ (numeral n'))) R.recN_succ).mpr
+            have R_numeral_n' : Red nat (numeral n') := by exact Red_numeral
             rcases Re'' with ⟨left, h0⟩; clear left
             specialize h0 (numeral n') R_numeral_n'
             rcases h0 with ⟨left, h0⟩; clear left
@@ -281,18 +282,18 @@ lemma all_R {e : Exp a} : R a e :=
 
 
 -- e ~ nbe a e
-lemma convr_nbe {e : Exp a} : convr e (nbe a e) := R_convr_nbe all_R
+lemma R_nbe {e : Exp a} : R e (nbe a e) := Red_R_nbe all_Red
 
 -- nbe a e = nbe a e' implies e ~ e'
-lemma completeness : nbe a e = nbe a e' → convr e e' :=
+lemma completeness : nbe a e = nbe a e' → R e e' :=
   by
   intro eq
-  -- convr-rewriting here
+  -- R-rewriting here
   -- e ~ nbe e = nbe e' ~ e'
-  -- "rewrite [convr_nbe, eq, ← convr_nbe]"
-  apply (convr_nbe).trans
+  -- "rewrite [R_nbe, eq, ← R_nbe]"
+  apply (R_nbe).trans
   rewrite [eq]; clear eq
-  exact convr_nbe.sym
+  exact R_nbe.symm
 
 -- e ~ e' ↔ nbe a e = nbe a e'
-lemma correctness {e e' : Exp a} : convr e e' ↔ nbe a e = nbe a e' := ⟨soundness, completeness⟩
+lemma correctness {e e' : Exp a} : R e e' ↔ nbe a e = nbe a e' := ⟨soundness, completeness⟩
